src/ExprT.v
@@ -2,8 +2,10 @@
  * This achieves a phase split between the 'well-formedness' of expressions
  * and their meaning
  *)
-Require Import List.
+Require Import List Bool.
 Require Import ExtLib.Data.HList.
+Require Import ExtLib.Tactics.EqDep.
+Require Import ExtLib.Core.RelDec.
 Require Import MirrorCore.ExprCore.
 
 Set Implicit Arguments.
@@ -12,11 +14,14 @@ Set Strict Implict.
 Section typed.
   Variable ts : types.
 
+  Definition typeof_func (f : function ts) : tfunction :=
+    {| tfenv := fenv f ; tftype := ftype f |}.
+
   Definition well_typed_func (tf : tfunction) (f : function ts) : bool :=
-    typ_eqb tf (ftype f).
+    (tfenv tf) ?[ eq ] (fenv f) && typ_eqb (tftype tf) (ftype f).
 
   Definition typeof_funcs : functions ts -> tfunctions :=
-    map (@ftype _).
+    map typeof_func.
 
   Fixpoint well_typed_funcs (tfs : tfunctions) (fs : functions ts) : bool :=
     match tfs , fs with
@@ -48,7 +53,11 @@ Section typed.
       | Func f ts =>
         match nth_error fs f with
           | None => None
-          | Some r => Some (instantiate_typ ts r)
+          | Some r => 
+            if EqNat.beq_nat (length ts) (tfenv r) then
+              Some (instantiate_typ (rev ts) (tftype r))
+            else
+              None
         end
       | App e es =>
         match typeof_expr var_env e with
@@ -60,6 +69,23 @@ Section typed.
           | None => None
           | Some t' => Some (tvArr t t')
         end
+      | Equal t e1 e2 => 
+        match typeof_expr var_env e1 with
+          | Some t' =>
+            if typ_eqb t t' then 
+              match typeof_expr var_env e2 with
+                | Some t' =>
+                  if typ_eqb t t' then Some tvProp else None
+                | None => None
+              end
+            else None
+          | None => None
+        end
+      | Not e =>
+ match typeof_expr var_env e with
+          | Some t' => if typ_eqb tvProp t' then Some tvProp else None
+          | None => None
+        end            
     end.
 
   Definition WellTyped_expr (var_env : tenv) (e : expr ts) (t : typ) : Prop :=
@@ -68,34 +94,84 @@ Section typed.
 End typed.
 
 Require Import ExtLib.Tactics.Consider.
+Require Import ExtLib.Data.ListNth.
 
-Theorem typ_eq_odec_None : forall t t', 
-  typ_eq_odec t t' = None -> t <> t'.
+Theorem nth_error_typeof_funcs : forall ts (fs : functions ts) n, 
+  nth_error (typeof_funcs fs) n = match nth_error fs n with
+                                    | None => None
+                                    | Some x => Some (typeof_func x)
+                                  end.
 Proof.
-Admitted.
-
-Theorem typ_eq_odec_None_refl : forall t,
-  typ_eq_odec t t = None -> False.
-Proof.
-  intros. apply typ_eq_odec_None in H. auto.
+  unfold typeof_funcs; intros.
+  rewrite nth_error_map. reflexivity.
 Qed.
 
-Theorem typ_eq_odec_Some_refl : forall t,
-  typ_eq_odec t t = Some refl_equal.
+Theorem nth_error_typeof_env : forall ts (fs : env ts) n, 
+  nth_error (typeof_env fs) n = match nth_error fs n with
+                                  | None => None
+                                  | Some x => Some (projT1 x)
+                                end.
 Proof.
-Admitted.
+  unfold typeof_env; intros.
+  rewrite nth_error_map. reflexivity.
+Qed.
 
-Theorem exprD_typof_expr_iff : forall ts (fs : functions ts) uenv venv e t,
-  WellTyped_expr (typeof_funcs fs) (typeof_env uenv) (typeof_env venv) e t ->
-  exists v, exprD fs uenv venv e t = Some v.
+Theorem typeof_typeof_expr : forall ts fs uenv e venv t, 
+  typeof_expr (ts := ts) (typeof_funcs fs) (typeof_env uenv) venv e = Some t ->
+  typeof fs uenv venv e = Some t.
 Proof.
-  unfold exprD, WellTyped_expr. intros.
-  cut (projT1 (split_env venv) = typeof_env venv).
-  destruct (split_env venv); simpl in *; intros; subst.
-  generalize dependent t; generalize dependent venv. 
+  induction e; simpl; intros;
+    repeat match goal with 
+             | [ H : _ |- _ ] => rewrite H in *
+             | [ H : Some _ = Some _ |- _ ] =>
+               inversion H; clear H; subst                 
+             | _ => rewrite nth_error_typeof_funcs in *
+             | _ => rewrite nth_error_typeof_env in *
+             | [ H : match ?X with _ => _ end = _ |- _ ] =>
+               (consider X; intros; try congruence); [ ]
+             | [ H : (if ?X then _ else _) = _ |- _ ] =>
+               (consider X; intros; try congruence); [ ]
+             | [ H : (if ?X then _ else _) = _ |- _ ] =>
+               solve [ consider X; intros; try congruence ]
+             | [ H : forall x, _ = _ -> _ |- _ ] =>
+               specialize (H _ eq_refl)
+             | |- None = Some _ => exfalso
+           end; simpl; try congruence; auto.
+  { eapply IHe in H0. rewrite H0. 
+    clear - H H1. revert H1. revert t0. induction H; simpl; intros; auto.
+    consider (typeof_expr (typeof_funcs fs) (typeof_env uenv) venv x); intros; try congruence.
+    erewrite H by eassumption.
+    destruct t0; auto. destruct (typ_eqb t0_1 t1); auto. }
+  { eapply IHe in H. rewrite H in *. reflexivity. }
+Qed.
+
+Theorem type_apply_length_equal : forall ts ft ts' n z fd,
+  length ts' = n ->
+  exists r, type_apply ts n ts' z ft fd = Some r.
+Proof.
+  induction ts'; simpl in *; intros; subst; simpl; eauto.
+  match goal with
+    [ |- exists x, match ?X with _ => _ end = _ ] =>
+    consider X
+  end; intros; eauto.
+  destruct (@IHts' (length ts') (typD ts z a :: z) (fd (typD ts z a)) eq_refl).  
+  simpl in *. clear - H H0.
+  match goal with
+    | [ H : ?X = None , H' : ?Y = Some _ |- _ ] =>
+      let H'' := fresh in
+        assert (H'' : X = Y) by reflexivity; congruence
+  end.
+Qed.
+
+Theorem exprD_typof_expr_iff' : forall ts (fs : functions ts) uenv e tvenv t,
+  typeof_expr (typeof_funcs fs) (typeof_env uenv) tvenv e = Some t ->
+  exists v, exprD' fs uenv tvenv e t = Some v.
+Proof.
+  unfold WellTyped_expr.
   induction e; simpl; intros;
     repeat match goal with
              | [ H : Some _ = Some _ |- _ ] => inversion H; clear H; subst
+             | _ => congruence
              | [ H : typ_eq_odec _ _ = None |- _ ] => 
                apply typ_eq_odec_None in H
              | |- context [ match ?X with _ => _ end ] =>
@@ -103,25 +179,48 @@ Proof.
                  | match _ with _ => _ end => fail 1
                  | _ => consider X; intros
                end
-           end; try solve [ eauto | exfalso; auto ].
-  { revert H0. 
-    match goal with
-      | |- match _ with _ => _ end ?X = _ -> _ =>
-        generalize X
+             | [ H : match ?X with _ => _ end = _ |- _ ] =>
+               (consider X; intros; try congruence); [ ]
+             | [ H : match ?X with _ => _ end = _ |- _ ] =>
+               solve [ consider X; intros; try congruence ]
+             | [ H : context [ if ?X then _ else _ ] |- _ ] =>
+               (consider X; intros; try congruence); [ ]
+             | [ H : _ = _ |- _ ] => rewrite H in *
+             | _ => rewrite nth_error_typeof_funcs in *
+             | _ => rewrite nth_error_typeof_env in *
+             | [ H : typeof_expr _ _ _ _ = Some _
+               , H' : typeof _ _ _ _ = None |- _ ] =>
+             eapply typeof_typeof_expr in H; congruence
+             | [ H : typ_eqb _ _ = true |- _ ] => apply typ_eqb_true in H; subst
+             | [ H : exists x, _ |- _ ] => destruct H
+             | [ H' : forall x y, typeof_expr _ _ _ ?X = Some _ -> _
+               , H : typeof_expr _ _ _ ?X = Some _ |- _ ] =>
+             specialize (H' _ _ H)
+             | [ |- exists x, None = Some _ ] => exfalso
+           end; try solve [ congruence | eauto | auto ].
+  { match goal with
+      | |- context [ @eq_refl _ ?X ] =>
+        generalize (@eq_refl _ X)
     end.
-    pattern (nth_error (typeof_env venv) v) at 2 3.
-    rewrite H. rewrite typ_eq_odec_Some_refl.
-    intros. congruence. }
-  { admit. }
-  { admit. }
-  { admit. }
-  { admit. }
-  { admit. }
-  { admit. }
-  { admit. }
-  { admit. }
-  { admit. }
-  { admit. }
-  { admit. }
-  { admit. }
+    pattern (nth_error tvenv v) at 2 3.
+    rewrite H.
+    rewrite typ_eq_odec_Some_refl.
+    intros. eauto. }
+  { destruct f0; simpl in *.  
+    eapply type_apply_length_equal with (fd := fdenote) in H2. rewrite H1 in H2. 
+    destruct H2; congruence. }
+  { revert H3. eapply typeof_typeof_expr in H0. rewrite H1 in H0.
+    inversion H0; clear H0; subst. rewrite H4 in H2. inversion H2; clear H2; subst.
+    clear - H. generalize dependent t2.
+    induction H; simpl; intros.
+    { inversion H3; clear H3; subst. rewrite typ_eq_odec_Some_refl. eauto. }
+    { consider (typeof_expr (typeof_funcs fs) (typeof_env uenv) tvenv x); intros; try congruence.
+      destruct t2; try congruence.
+      change (typ_eqb t2_1 t0) with (t2_1 ?[ eq ] t0) in *.
+      consider (t2_1 ?[ eq ] t0); intros; try congruence; subst.
+      eapply H in H1. destruct H1. rewrite H1. eauto. } }
+  { eapply typeof_typeof_expr in H0. rewrite H1 in H0.
+    inversion H0; clear H0; subst. congruence. }
+  { unfold lookupAs in *. rewrite H in *.
+    rewrite typ_eq_odec_Some_refl in H0. congruence. }
 Qed.
